% \documentclass[a4paper,10pt]{article}
\documentclass[a4paper,10pt]{scrartcl}

\usepackage[utf8]{inputenc}
\usepackage[fleqn]{amsmath}
\usepackage{amssymb}
\usepackage{mathtools}
\usepackage[left=2.5cm, right=2.5cm, top=2.5cm, bottom=2cm]{geometry}

\title{}
\author{}
\date{}

\pdfinfo{%
  /Title    ()
  /Author   ()
  /Creator  ()
  /Producer ()
  /Subject  ()
  /Keywords ()
}

\begin{document}

\noindent Let $x, y \in \mathbb{H}$, with
\begin{align*}
 x &= x_0 + x_1 \mathrm{i} + x_2 \mathrm{j} + x_3 \mathrm{k} \\
 y &= y_0 + y_1 \mathrm{i} + y_2 \mathrm{j} + y_3 \mathrm{k}
\end{align*}

\noindent Using the following rules:
\begin{align}
 \mathrm{i}^2 = \mathrm{j}^2 = \mathrm{k}^2 = -1
\end{align}
\begin{align}
 \mathrm{i} \mathrm{j} = +\mathrm{k},\quad \mathrm{j} \mathrm{k} = +\mathrm{i},\quad \mathrm{k} \mathrm{i} = +\mathrm{j} \\
 \mathrm{j} \mathrm{i} = -\mathrm{k},\quad \mathrm{k} \mathrm{j} = -\mathrm{i},\quad \mathrm{i} \mathrm{k} = -\mathrm{j} \tag{$\overline{2}$}
\end{align}
\begin{align}
 \mathrm{ijk} = 1
\end{align}

\noindent one can express $xy$ as
{\setlength{\mathindent}{\mathindent / 2}
\begin{gather*}
 \begin{alignat*}{1}
  x y ={}& (x_0 + x_1 \mathrm{i} + x_2 \mathrm{j} + x_3 \mathrm{k}) (y_0 + y_1 \mathrm{i} + y_2 \mathrm{j} + y_3 \mathrm{k})
 \end{alignat*} \\
 \begin{alignat*}{4}
  \phantom{xy}={}&\phantom{{}+{}} x_0 y_0 && {}+ x_0 y_1 \mathrm{i} && {}+ x_0 y_2 \mathrm{j} && {}+ x_0 y_3 \mathrm{k} \\
  &+ x_1 y_0 \mathrm{i} && {}+ x_1 y_1 \mathrm{i}^2 && {}+ x_1 y_2 \mathrm{ij}  && {}+ x_1 y_3 \mathrm{ik} \\
  &+ x_2 y_0 \mathrm{j} && {}+ x_2 y_1 \mathrm{ji}  && {}+ x_2 y_2 \mathrm{j}^2 && {}+ x_2 y_3 \mathrm{jk} \\
  &+ x_3 y_0 \mathrm{k} && {}+ x_3 y_1 \mathrm{ki}  && {}+ x_3 y_2 \mathrm{kj}  && {}+ x_3 y_3 \mathrm{k}^2
 \end{alignat*} \\
 \begin{alignat*}{4}
  \phantom{xy}={}&\phantom{{}+{}} x_0 y_0 && {}+ x_0 y_1 \mathrm{i} && {}+ x_0 y_2 \mathrm{j} && {}+ x_0 y_3 \mathrm{k} \\
  &+ x_1 y_0 \mathrm{i} && {}- x_1 y_1 && {}+ x_1 y_2 \mathrm{k}  && {}- x_1 y_3 \mathrm{j} \\
  &+ x_2 y_0 \mathrm{j} && {}- x_2 y_1 \mathrm{k}  && {}- x_2 y_2 && {}+ x_2 y_3 \mathrm{i} \\
  &+ x_3 y_0 \mathrm{k} && {}+ x_3 y_1 \mathrm{j}  && {}- x_3 y_2 \mathrm{i}  && {}- x_3 y_3
 \end{alignat*} \\
 \begin{alignat*}{5}
  \phantom{xy}={}&\phantom{{}+{}} (x_0 y_0 && {}- x_1 y_1 && {}- x_2 y_2 && {}- x_3 y_3) \\
  &+ (x_0 y_1 && {}+ x_1 y_0 && {}+ x_2 y_3 && {}- x_3 y_2) && \mathrm{i} \\
  &+ (x_0 y_2 && {}- x_1 y_3 && {}+ x_2 y_0 && {}+ x_3 y_1) && \mathrm{j} \\
  &+ (x_0 y_3 && {}+ x_1 y_2 && {}- x_2 y_1 && {}+ x_3 y_0) && \mathrm{k}
 \end{alignat*}
\end{gather*}}

\end{document}
